Set up inductive hypothesis structure (with sorry's)

ParserCombinators/Basic.lean
@@ -245,9 +245,24 @@ private def many_run (p : Parser a) (h : not_nullable p) (input : Str) : Option 
   | none => some ([], input)
 termination_by input.length
 
+theorem many_run_decreases (p : Parser a) (h : not_nullable p) : ∀ (s : Str) (res : List a × Str), many_run p h s = some res → res.2 <:+ s := by {
+  intro s
+  induction s with
+  | nil =>
+    simp only [List.suffix_nil, Prod.forall]
+    sorry
+  | cons c s' ih =>
+    cases h1 : p.run (c :: s') with
+    | none =>
+      simp only [Prod.forall]
+      sorry
+    | some => sorry
+}
+
 def many (p : Parser a) (h : not_nullable p) : Parser (List a) where
   run := many_run p h
-  decreases := by sorry
+  decreases := by { sorry
+  }
 
 def many1 (p : Parser a) (h : not_nullable p) : Parser (List a) :=
   map (fun x => x.1 :: x.2) (concat p (many p h))
